prooftactic.md
@@ -1,3 +1,6 @@
 To debug, put a breakpoint on the first Left constructor in trace_solve_tac
 Then, you can evaluate get_tacs data0 in the debugger and try to find its origin.
+It seems better to look at the variable tag in solve (trac_solve_tac)
 For instance, the constructor BlackBoxTac is used in CogentHelper
+
+
